testdata/out/pg/github_com/mjschwenne/grackle/testdata/out/go/error_gk.v
@@ -20,6 +20,8 @@ Section names.
 
 Class GlobalAddrs :=
 {
+  Name : loc;
+  Value : loc;
 }.
 
 Context `{!GlobalAddrs}.
@@ -27,6 +29,8 @@ Context `{hG: heapGS Σ, !ffi_semantics _ _}.
 Context `{!goGlobalsGS Σ}.
 
 Definition var_addrs : list (go_string * loc) := [
+    ("Name"%go, Name);
+    ("Value"%go, Value)
   ].
 
 Global Instance is_pkg_defined_instance : IsPkgDefined error_gk :=
@@ -35,7 +39,24 @@ Global Instance is_pkg_defined_instance : IsPkgDefined error_gk :=
 |}.
 
 Definition own_allocated : iProp Σ :=
-True.
+  "HName" ∷ Name ↦ (default_val loc) ∗
+  "HValue" ∷ Value ↦ (default_val loc).
+
+Global Instance wp_globals_get_Name : 
+  WpGlobalsGet error_gk "Name" Name (is_pkg_defined error_gk).
+Proof. apply wp_globals_get'. reflexivity. Qed.
+
+Global Instance wp_globals_get_Value : 
+  WpGlobalsGet error_gk "Value" Value (is_pkg_defined error_gk).
+Proof. apply wp_globals_get'. reflexivity. Qed.
+
+Global Instance wp_method_call_E_String :
+  WpMethodCall error_gk "E" "String" _ (is_pkg_defined error_gk) :=
+  ltac:(apply wp_method_call'; reflexivity).
+
+Global Instance wp_method_call_E'ptr_String :
+  WpMethodCall error_gk "E'ptr" "String" _ (is_pkg_defined error_gk) :=
+  ltac:(apply wp_method_call'; reflexivity).
 
 End names.
 End error_gk.
